Fixed Canonicalisation Errors
Fixed the type errors in canonicalisation, didn't fix the proofs yet
but it's a start

Canonicalization.thy
@@ -2,37 +2,35 @@ section \<open>Canonicalization optimisation transformations\<close>
 
 theory Canonicalization
   imports 
-    IREval
+    IRGraphFrames
     IRStepObj
+    
 begin
-(*
-declare [[show_types]]
-declare [[show_sorts]]
-declare [[show_consts]]
-*)
+
+
 lemma eval_const_node:
-  assumes xn: "kind g x = ConstantNode xv"
-  shows "g m \<turnstile> x (kind g x) \<mapsto> (IntVal xv)"
+  assumes xn: "kind g x = Some (ConstantNode xv)"
+  shows "g m \<turnstile> x (the (kind g x)) \<mapsto> (IntVal xv)"
   using xn eval.ConstantNode by simp
 
 lemma eval_add_node: 
-  assumes x: "g m \<turnstile> x (kind g x) \<mapsto> IntVal(xv)"
-  assumes y: "g m \<turnstile> y (kind g y) \<mapsto> IntVal(yv)"
+  assumes x: "g m \<turnstile> x (the (kind g x)) \<mapsto> IntVal(xv)"
+  assumes y: "g m \<turnstile> y (the (kind g y)) \<mapsto> IntVal(yv)"
   shows "g m \<turnstile> z (AddNode x y) \<mapsto> IntVal(xv+yv)"
   using eval.AddNode x y by blast
 
 lemma add_const_nodes:
-  assumes xn: "kind g x = ConstantNode xv"
-  assumes yn: "kind g y = ConstantNode yv"
-  assumes zn: "kind g z = AddNode x y"
-  assumes wn: "kind g w = ConstantNode (xv+yv)"
-  assumes ez: "g m \<turnstile> z (kind g z) \<mapsto> (IntVal v1)"
-  assumes ew: "g m \<turnstile> w (kind g w) \<mapsto> (IntVal v2)"
+  assumes xn: "kind g x = Some (ConstantNode xv)"
+  assumes yn: "kind g y = Some (ConstantNode yv)"
+  assumes zn: "kind g z = Some (AddNode x y)"
+  assumes wn: "kind g w = Some (ConstantNode (xv+yv))"
+  assumes ez: "g m \<turnstile> z (the (kind g z)) \<mapsto> (IntVal v1)"
+  assumes ew: "g m \<turnstile> w (the (kind g w)) \<mapsto> (IntVal v2)"
   shows "v1 = v2"
 proof -
-  have zv: "g m \<turnstile> z (kind g z) \<mapsto> IntVal(xv+yv)"
+  have zv: "g m \<turnstile> z (the (kind g z)) \<mapsto> IntVal(xv+yv)"
     using eval.AddNode eval_const_node xn yn zn by simp
-  have wv: "g m \<turnstile> w (kind g w) \<mapsto> IntVal(xv+yv)"
+  have wv: "g m \<turnstile> w (the (kind g w)) \<mapsto> IntVal(xv+yv)"
     using eval_const_node wn by auto
   show ?thesis using evalDet zv wv
     using ew ez by blast
@@ -41,13 +39,13 @@ qed
 text_raw \<open>\Snip{CreateAddNode}%\<close>
 fun create_add :: "IRGraph \<Rightarrow> ID \<Rightarrow> ID \<Rightarrow> IRNode" where 
   "create_add g x y = 
-    (case kind g x of 
+    (case the (kind g x) of 
       ConstantNode xv \<Rightarrow> 
-        (case kind g y of
+        (case the (kind g y) of
           ConstantNode yv \<Rightarrow> ConstantNode (xv+yv) | 
           _ \<Rightarrow> if xv = 0 then RefNode y else AddNode x y
         ) |
-      _ \<Rightarrow> (case kind g y of
+      _ \<Rightarrow> (case the (kind g y) of
             ConstantNode yv \<Rightarrow> 
               if yv = 0 then RefNode x else AddNode x y |
             _ \<Rightarrow> AddNode x y
@@ -57,8 +55,8 @@ text_raw \<open>\EndSnip\<close>
 
 text_raw \<open>\Snip{AddNodeCreate}%\<close>
 lemma add_node_create:
-  assumes xv: "g m \<turnstile> x (kind g x) \<mapsto> IntVal(xv)"
-  assumes yv: "g m \<turnstile> y (kind g y) \<mapsto> IntVal(yv)"
+  assumes xv: "g m \<turnstile> x (the (kind g x)) \<mapsto> IntVal(xv)"
+  assumes yv: "g m \<turnstile> y (the (kind g y)) \<mapsto> IntVal(yv)"
   shows 
     "(g m \<turnstile> nid (AddNode x y) \<mapsto> IntVal(xv+yv)) \<and>
      (g m \<turnstile> nid (create_add g x y) \<mapsto> IntVal(xv+yv))"
@@ -71,20 +69,20 @@ proof -
   have refy: "\<forall>zy. (g m \<turnstile> zy (RefNode y) \<mapsto> IntVal yv)"
     using eval.RefNode yv by blast 
   have ce: "g m \<turnstile> nid (create_add g x y) \<mapsto> IntVal(xv+yv)"
-  proof (cases "\<exists>xvv. kind g x  = ConstantNode xvv")
+  proof (cases "\<exists>xvv. kind g x  = Some (ConstantNode xvv)")
     case xvvn: True
-    have xvv: "kind g x = ConstantNode xv" 
+    have xvv: "kind g x = Some (ConstantNode xv)" 
       using ConstantNode evalDet xv eval.ConstantNode xvvn by fastforce
     have cv1: "create_add g x y = 
-                (case kind g y of
+                (case the (kind g y) of
                  ConstantNode yvv \<Rightarrow> ConstantNode (xv+yvv) | 
                  _ \<Rightarrow> if xv = 0 then RefNode y else AddNode x y
                 )"
       using xvv by simp
     thus ?thesis 
-    proof (cases "\<exists>yvv. kind g y = ConstantNode yvv")
+    proof (cases "\<exists>yvv. the (kind g y) = ConstantNode yvv")
       case True
-        have yvv: "kind g y = ConstantNode yv"
+        have yvv: "the (kind g y) = ConstantNode yv"
         using ConstantNode evalDet yv eval.ConstantNode True by fastforce
       then show ?thesis
       proof -
@@ -96,18 +94,16 @@ proof -
       qed
     next
       case not_const_y:False
-      have not_const: "\<forall>yvv. kind g y \<noteq> ConstantNode yvv"
+      have not_const: "\<forall>yvv. the (kind g y) \<noteq> ConstantNode yvv"
         using not_const_y by blast
-      have cv_case: "(case kind g y of
+      then have cv_case: "(case the (kind g y) of
                  ConstantNode yvv \<Rightarrow> ConstantNode (xv+yvv) | 
                  _ \<Rightarrow> if xv = 0 then RefNode y else AddNode x y
                 ) = (if xv = 0 then RefNode y else AddNode x y)"
         apply (simp add: not_const)
         apply (cases "xv = 0"; auto)
-        apply (cases "case IRGraph.snd g y of None \<Rightarrow> NoNode | Some n \<Rightarrow> n"; auto)
         using not_const_y apply auto[1]
-        apply (cases "case IRGraph.snd g y of None \<Rightarrow> NoNode | Some n \<Rightarrow> n"; auto)
-        using not_const_y by auto
+        using not_const_y sorry
       have cv2: "create_add g x y = (if xv = 0 then RefNode y else AddNode x y)"
           using cv1 xvvn not_const_y xvv cv_case by simp
       then show ?thesis
@@ -124,33 +120,31 @@ proof -
   next
     case xnotconst: False
     then show ?thesis 
-    proof (cases "\<exists>yvv. kind g y = ConstantNode yvv")
+    proof (cases "\<exists>yvv. kind g y = Some (ConstantNode yvv)")
       case yvvn: True
-      have yvv: "kind g y = ConstantNode yv"
+      have yvv: "kind g y = Some (ConstantNode yv)"
         using ConstantNode evalDet yv eval.ConstantNode yvvn by fastforce 
       have cv3: "create_add g x y = (if yv = 0 then RefNode x else AddNode x y)"
         using yvv yvvn apply auto
-         apply (cases "case IRGraph.snd g x of None \<Rightarrow> NoNode | Some n \<Rightarrow> n"; auto)
         using xnotconst apply auto[1]
-        apply (cases "case IRGraph.snd g x of None \<Rightarrow> NoNode | Some n \<Rightarrow> n"; auto)
-        using xnotconst by auto
+        using xnotconst sorry
       then show ?thesis using cv3 ae yvv xv eval.RefNode by auto
     next 
       case ynotconst: False
-      have yvv: "kind g y \<noteq> ConstantNode yv"
+      have yvv: "kind g y \<noteq> Some (ConstantNode yv)"
         using ynotconst by simp
-      have xvv: "kind g x \<noteq> ConstantNode xv"
+      have xvv: "kind g x \<noteq> Some (ConstantNode xv)"
         using xnotconst by simp
-      have unwrapy: "(case kind g y of 
+      have unwrapy: "(case the (kind g y) of 
               ConstantNode yv \<Rightarrow> if yv = 0 then RefNode x else AddNode x y
             | _ \<Rightarrow> AddNode x y) = AddNode x y"
-        apply (cases "kind g y"; auto)
-        using ynotconst by auto
+        apply (cases "the (kind g y)"; auto)
+        using ynotconst sorry
       have cv4: "create_add g x y = AddNode x y"
         using xvv yvv unwrapy apply auto
         apply (cases "kind g x"; auto)
         using xnotconst apply auto[1]
-        using xnotconst by auto
+        using xnotconst sorry
       thus ?thesis using cv4 ae by simp
     qed
   qed
@@ -162,7 +156,7 @@ text_raw \<open>\Snip{CreateIfNode}%\<close>
 fun create_if :: "IRGraph \<Rightarrow> ID \<Rightarrow> ID \<Rightarrow> ID \<Rightarrow> IRNode"
   where 
   "create_if g cond tb fb = 
-    (case kind g cond of 
+    (case the (kind g cond) of 
       ConstantNode condv \<Rightarrow> 
         RefNode (if (val_to_bool condv) then tb else fb) |
       _ \<Rightarrow> (if tb = fb then
@@ -186,438 +180,16 @@ inductive stutter:: "Program \<Rightarrow> Signature \<Rightarrow> MapState \<Ri
    \<Longrightarrow> g s m \<turnstile> nid \<leadsto> nid'"
 text_raw \<open>\EndSnip\<close>
 
-inductive eval_uses:: "IRGraph \<Rightarrow> ID \<Rightarrow> ID \<Rightarrow> bool"
-  for g where
+lemma add_node_lookup:
+  assumes "g' = add_node nid k g"
+  shows "kind g' nid = Some k"
+  using assms unfolding add_node.simps
+  using Rep_IRGraph_inverse kind.transfer by auto
 
-  "\<lbrakk>kind g nid = n;
-    inputs_of n = ls;
-    nid' \<in> set ls\<rbrakk>
-    \<Longrightarrow> eval_uses g nid nid'" |
-
-  "\<lbrakk>eval_uses g nid nid';
-    eval_uses g nid' nid''\<rbrakk>
-    \<Longrightarrow> eval_uses g nid nid''"
-
-fun eval_usages :: "IRGraph \<Rightarrow> ID \<Rightarrow> ID set" where
-  "eval_usages g nid = set (filter (eval_uses g nid) (sorted_list_of_set (ids g)))"
-
-lemma eval_usages[simp]:
-  assumes "us = eval_usages g nid"
-  assumes "nid' \<in> ids g"
-  shows "eval_uses g nid nid' \<longleftrightarrow> nid' \<in> us" (is "?P \<longleftrightarrow> ?Q")
-  using assms eval_usages.simps by simp
-
-lemma inputs_are_uses:
-  assumes "nid' \<in> set (inputs_of (kind g nid))"
-  shows "eval_uses g nid nid'"
-  using assms eval_uses.intros(1) by blast
-
-lemma inputs_are_usages:
-  assumes "nid' \<in> set (inputs_of (kind g nid))"
-  assumes "nid' \<in> ids g"
-  shows "nid' \<in> eval_usages g nid"
-  using assms(1) assms(2) eval_usages inputs_are_uses by blast
-
-lemma usage_includes_inputs:
-  assumes "us = eval_usages g nid"
-  assumes "ls = set (inputs_of (kind g nid))"
-  assumes "ls \<subseteq> ids g"
-  shows "ls \<subseteq> us"
-  using inputs_are_usages eval_usages
-  using assms(1) assms(2) assms(3) by blast
-
-
-lemma kind_uneffected:
-  assumes oldnid: "nid \<in> ids g"
-  assumes newnid: "newnid \<notin> ids g"
-  assumes modg: "modg = add_node newnid anyk g"
-  shows "(kind g nid) = (kind modg nid)"
-proof -
-  have uneq: "nid \<noteq> newnid"
-    using newnid oldnid by blast
-  show ?thesis using uneq modg
-    apply (simp add: Abs_IRGraph_inverse snd.rep_eq)
-    using irgraph_dom
-    by (smt finsert_iff fun_upd_same fun_upd_triv fun_upd_twist ids.simps irgraph_dom_inv irgraph_dom_x irgraph_rng notin_fset option.discI snd.rep_eq)
-qed
-
-lemma kind_uneffected_uneq:
-  assumes "nid \<noteq> newnid"
-  assumes modg: "modg = add_node newnid anyk g"
-  shows "(kind g nid) = (kind modg nid)"
-proof -
-  show ?thesis using assms modg
-    apply (simp add: Abs_IRGraph_inverse snd.rep_eq)
-    using irgraph_dom
-    by (smt finsert_iff fun_upd_same fun_upd_triv fun_upd_twist ids.simps irgraph_dom_inv irgraph_dom_x irgraph_rng notin_fset option.discI snd.rep_eq)
-qed
-
-lemma not_in_no_val:
-  assumes "nid \<notin> ids g"
-  shows "\<not>(g m \<turnstile> nid (kind g nid) \<mapsto> x)"
-proof -
-  have kind: "(kind g nid) = NoNode"
-    using assms irgraph_dom_inv by auto
-  show ?thesis using kind
-    by auto
-qed
-
-lemma add_implies_kind:
-  assumes add: "gup = add_node nid k g"
-  shows "kind gup nid = k"
-proof -
-  have isin: "nid \<in> dom (snd gup)"
-    using add apply simp
-    by (smt domIff dom_fun_upd finsert_iff ids.simps insert_iff irgraph_dom_inv irgraph_dom_x irgraph_rng notin_fset option.discI)
-  show ?thesis using isin add apply simp
-    by (smt finsert_iff fun_upd_apply ids.simps irgraph_dom_inv irgraph_dom_x irgraph_rng notin_fset option.case_eq_if option.discI option.sel)
-qed
-
-fun changes :: "ID \<Rightarrow> IRGraph \<Rightarrow> IRGraph \<Rightarrow> bool" where
-  "changes nid g1 g2 = ((kind g1 nid) \<noteq> (kind g2 nid))"
-
-lemma add_node_changes:
-  assumes "nid \<notin> ids g1"
-  assumes "n \<noteq> NoNode"
-  assumes "g2 = add_node nid n g1"
-  shows "changes nid g1 g2"
-  using add_implies_kind assms(1) assms(2) assms(3) irgraph_dom_inv by auto
-
-lemma remove_node_effect:
-  assumes "g2 = remove_node nid g1"
-  shows "kind g2 nid = NoNode"
-  using Rep_IRGraph assms fst.rep_eq snd.rep_eq by auto
-
-lemma remove_node_changes:
-  assumes "nid \<in> ids g1"
-  assumes "kind g1 nid \<noteq> NoNode"
-  assumes "g2 = remove_node nid g1"
-  shows "changes nid g1 g2"
-  using assms(2) assms(3) remove_node_effect by auto
-
-lemma kind_floats:
-  assumes "g1 m \<turnstile> nid (kind g1 nid) \<mapsto> v1"
-  shows "is_floating_node (kind g1 nid)"
-  using assms evalFloating by blast
-
-lemma unchanged_implies_unchanged_inputs:
-  assumes "\<forall> nid' \<in> (eval_usages g1 nid) . \<not>(changes nid' g1 g2)"
-  shows "\<forall> nid' \<in> (eval_usages g1 nid) . (\<forall> nid'' \<in> (eval_usages g1 nid') . \<not>(changes nid'' g1 g2))"
-  by (metis assms eval_usages.simps eval_uses.intros(2) filter_set member_filter)
-
-lemma stay_same:
-  assumes "\<not>(changes nid g1 g2)"
-  assumes "\<forall> nid' \<in> (eval_usages g1 nid) . \<not>(changes nid' g1 g2)"
-  assumes "g1 m \<turnstile> nid (kind g1 nid) \<mapsto> v1"
-  shows "g2 m \<turnstile> nid (kind g2 nid) \<mapsto> v1" 
-proof -
-  have kind_same: "kind g1 nid = kind g2 nid"
-    using assms(1) by auto
-
-  show ?thesis using assms(3) assms(1) assms(2) kind_same
-proof (induct m nid "kind g1 nid" v1 arbitrary: nid rule: "eval.induct")
-  case const: (ConstantNode val c)
-  then have "kind g2 nid = (ConstantNode c)"
-    using kind_same by presburger
-  then show ?case
-    by (simp add: const.hyps(1) eval.ConstantNode)
-next
-  case param: (ParameterNode val m i nid)
-  show ?case
-    using eval.ParameterNode param.hyps(1) param.hyps(2) param.prems(3) by fastforce
-next
-  case phi: (PhiNode val m nid uu)
-  then have kind: "kind g2 nid = (PhiNode uu)"
-    by presburger
-  then have "g1 m \<turnstile> nid (kind g1 nid) \<mapsto> val"
-    using PhiNode phi.hyps(1) sorry
-  then show ?case
-    using PhiNode kind phi.prems(3) by auto
-next
-  case (ValuePhiNode val m nid uv uw)
-  then have kind: "kind g2 nid = (ValuePhiNode uv uw)"
-    by presburger
-  then have "g1 m \<turnstile> nid (kind g1 nid) \<mapsto> val"
-    sorry
-  then show ?case
-    using ValuePhiNode.prems(3) kind eval.ValuePhiNode by auto
-next
-  case (ValueProxyNode m c val nid u)
-  then have "g2 m \<turnstile> c (kind g2 c) \<mapsto> val"
-    by (smt changes.simps eval_usages.simps eval_uses.intros(2) filter_set inputs_are_usages inputs_of.simps list.set_intros(1) member_filter not_in_no_val set_subset_Cons subsetD)
-  then show ?case
-    by (metis ValueProxyNode.hyps(3) ValueProxyNode.prems(3) eval.ValueProxyNode)
-next
-  case (AbsNode m x v nid)
-  then have "g2 m \<turnstile> x (kind g2 x) \<mapsto> IntVal v"
-    by (metis changes.elims(3) inputs_are_usages inputs_of_AbsNode list.set_intros(1) not_in_no_val unchanged_implies_unchanged_inputs)
-  then show ?case
-    using AbsNode.hyps(3) AbsNode.prems(3) eval.AbsNode by fastforce
-next
-  case (NegateNode m x v nid)
-  then have "g1 m \<turnstile> x (kind g1 x) \<mapsto> IntVal v"
-    by presburger
-  then have "g2 m \<turnstile> x (kind g2 x) \<mapsto> IntVal v"
-    using unchanged_implies_unchanged_inputs assms
-    by (metis NegateNode.hyps(2) NegateNode.hyps(3) NegateNode.prems(2) changes.elims(3) inputs_are_usages inputs_of_NegateNode list.set_intros(1) not_in_no_val)
-  then show ?case
-    using NegateNode.hyps(3) NegateNode.prems(3) eval.NegateNode by fastforce
-next
-  case (AddNode m x v1 y v2 nid)
-  then have "g1 m \<turnstile> x (kind g1 x) \<mapsto> IntVal v1"
-    by blast
-  then have v1: "g2 m \<turnstile> x (kind g2 x) \<mapsto> IntVal v1"
-    using unchanged_implies_unchanged_inputs
-    by (metis AddNode.hyps(2) AddNode.hyps(5) AddNode.prems(2) changes.elims(3) inputs_are_usages inputs_of_AddNode list.set_intros(1) not_in_no_val)
-  have "g1 m \<turnstile> y (kind g1 y) \<mapsto> IntVal v2"
-    using AddNode.hyps(3) by simp
-  then have v2: "g2 m \<turnstile> y (kind g2 y) \<mapsto> IntVal v2"
-    using unchanged_implies_unchanged_inputs
-    by (metis AddNode.hyps(4) AddNode.hyps(5) AddNode.prems(2) changes.elims(3) in_mono inputs_are_usages inputs_of_AddNode list.set_intros(1) not_in_no_val set_subset_Cons)
-  then show ?case using v1 v2
-    using AddNode.hyps(5) AddNode.prems(3) eval.AddNode by fastforce
-next
-  case (SubNode m x v1 y v2 nid)
-  then have "g1 m \<turnstile> x (kind g1 x) \<mapsto> IntVal v1"
-    by blast
-  then have v1: "g2 m \<turnstile> x (kind g2 x) \<mapsto> IntVal v1"
-    by (metis SubNode.hyps(2) SubNode.hyps(5) SubNode.prems(2) changes.elims(3) inputs_are_usages inputs_of_SubNode list.set_intros(1) not_in_no_val unchanged_implies_unchanged_inputs)
-  have "g1 m \<turnstile> y (kind g1 y) \<mapsto> IntVal v2"
-    using SubNode.hyps(3) by auto
-  then have v2: "g2 m \<turnstile> y (kind g2 y) \<mapsto> IntVal v2"
-    by (metis SubNode.hyps(4) SubNode.hyps(5) SubNode.prems(2) changes.elims(3) in_mono inputs_are_usages inputs_of_SubNode list.set_intros(1) not_in_no_val set_subset_Cons unchanged_implies_unchanged_inputs)
-  then show ?case using v1 v2
-    using SubNode.hyps(5) SubNode.prems(3) eval.SubNode by fastforce
-next
-  case node: (MulNode m x v1 y v2 nid)
-  then have "g1 m \<turnstile> x (kind g1 x) \<mapsto> IntVal v1"
-    by blast
-  then have v1: "g2 m \<turnstile> x (kind g2 x) \<mapsto> IntVal v1"
-    by (metis changes.elims(3) inputs_are_usages inputs_of_MulNode list.set_intros(1) node.hyps(2) node.hyps(5) node.prems(2) not_in_no_val unchanged_implies_unchanged_inputs)
-  have "g1 m \<turnstile> y (kind g1 y) \<mapsto> IntVal v2"
-    using node.hyps(3) by auto
-  then have v2: "g2 m \<turnstile> y (kind g2 y) \<mapsto> IntVal v2"
-  by (metis changes.elims(3) in_mono inputs_are_usages inputs_of_MulNode list.set_intros(1) node.hyps(4) node.hyps(5) node.prems(2) not_in_no_val set_subset_Cons unchanged_implies_unchanged_inputs)
-    then show ?case using v1 v2
-    using node.hyps(5) node.prems(3) eval.MulNode by fastforce
-next
-  case node: (AndNode m x v1 y v2 nid)
-  then have "g1 m \<turnstile> x (kind g1 x) \<mapsto> IntVal v1"
-    by blast
-  then have v1: "g2 m \<turnstile> x (kind g2 x) \<mapsto> IntVal v1"
-    by (metis changes.elims(3) inputs_are_usages inputs_of_AndNode list.set_intros(1) node.hyps(2) node.hyps(5) node.prems(2) not_in_no_val unchanged_implies_unchanged_inputs)
-  have "g1 m \<turnstile> y (kind g1 y) \<mapsto> IntVal v2"
-    using node.hyps(3) by auto
-  then have v2: "g2 m \<turnstile> y (kind g2 y) \<mapsto> IntVal v2"
-    by (metis (no_types, lifting) changes.simps eval_usages.simps eval_uses.intros(2) filter_set in_set_member inputs_are_usages inputs_of_AndNode member_filter member_rec(1) node.hyps(4) node.hyps(5) node.prems(2) not_in_no_val)
-  then show ?case using v1 v2
-    using node.hyps(5) node.prems(3) eval.AndNode by fastforce
-next
-  case node: (OrNode m x v1 y v2 nid)
-  then have "g1 m \<turnstile> x (kind g1 x) \<mapsto> IntVal v1"
-    by blast
-  then have v1: "g2 m \<turnstile> x (kind g2 x) \<mapsto> IntVal v1"
-    by (metis changes.elims(3) inputs_are_usages inputs_of_OrNode list.set_intros(1) node.hyps(2) node.hyps(5) node.prems(2) not_in_no_val unchanged_implies_unchanged_inputs)
-  have "g1 m \<turnstile> y (kind g1 y) \<mapsto> IntVal v2"
-    using node.hyps(3) by auto
-  then have v2: "g2 m \<turnstile> y (kind g2 y) \<mapsto> IntVal v2"
-    by (metis (no_types, lifting) changes.simps eval_usages.simps eval_uses.intros(2) filter_set in_set_member inputs_are_usages inputs_of_OrNode member_filter member_rec(1) node.hyps(4) node.hyps(5) node.prems(2) not_in_no_val)
-  then show ?case using v1 v2
-    using node.hyps(5) node.prems(3) eval.OrNode by fastforce
-next
-  case node: (XorNode m x v1 y v2 nid)
-  then have "g1 m \<turnstile> x (kind g1 x) \<mapsto> IntVal v1"
-    by blast
-  then have v1: "g2 m \<turnstile> x (kind g2 x) \<mapsto> IntVal v1"
-    by (metis changes.elims(3) inputs_are_usages inputs_of_XorNode list.set_intros(1) node.hyps(2) node.hyps(5) node.prems(2) not_in_no_val unchanged_implies_unchanged_inputs)
-  have "g1 m \<turnstile> y (kind g1 y) \<mapsto> IntVal v2"
-    using node.hyps(3) by auto
-  then have v2: "g2 m \<turnstile> y (kind g2 y) \<mapsto> IntVal v2"
-    by (metis changes.elims(3) in_mono inputs_are_usages inputs_of_XorNode list.set_intros(1) node.hyps(4) node.hyps(5) node.prems(2) not_in_no_val set_subset_Cons unchanged_implies_unchanged_inputs)
-  then show ?case using v1 v2
-    using node.hyps(5) node.prems(3) eval.XorNode by fastforce
-next
-  case node: (IntegerEqualsNode m x v1 y v2 val nid)
-  then have "g1 m \<turnstile> x (kind g1 x) \<mapsto> IntVal v1"
-    by blast
-  then have v1: "g2 m \<turnstile> x (kind g2 x) \<mapsto> IntVal v1"
-    by (metis changes.elims(3) inputs_are_usages inputs_of_IntegerEqualsNode list.set_intros(1) node.hyps(2) node.hyps(6) node.prems(2) not_in_no_val unchanged_implies_unchanged_inputs)
-  have "g1 m \<turnstile> y (kind g1 y) \<mapsto> IntVal v2"
-    using node.hyps(3) by auto
-  then have v2: "g2 m \<turnstile> y (kind g2 y) \<mapsto> IntVal v2"
-    by (metis (no_types, lifting) changes.simps eval_usages.simps eval_uses.intros(2) filter_set in_set_member inputs_are_usages inputs_of_IntegerEqualsNode member_filter member_rec(1) node.hyps(4) node.hyps(6) node.prems(2) not_in_no_val)
-  then show ?case using v1 v2
-    using IntegerEqualsNode node.hyps(5) node.hyps(6) node.prems(3) by fastforce
-next
-  case node: (IntegerLessThanNode m x v1 y v2 val nid)
-  then have "g1 m \<turnstile> x (kind g1 x) \<mapsto> IntVal v1"
-    by blast
-  then have v1: "g2 m \<turnstile> x (kind g2 x) \<mapsto> IntVal v1"
-    by (metis (no_types, lifting) changes.simps eval_usages.simps eval_uses.intros(2) filter_set inputs_are_usages inputs_of_IntegerLessThanNode list.set_intros(1) member_filter node.hyps(2) node.hyps(6) node.prems(2) not_in_no_val)
-  have "g1 m \<turnstile> y (kind g1 y) \<mapsto> IntVal v2"
-    using node.hyps(3) by auto
-  then have v2: "g2 m \<turnstile> y (kind g2 y) \<mapsto> IntVal v2"
-    by (metis (no_types, lifting) changes.simps eval_usages.simps eval_uses.intros(2) filter_set in_set_member inputs_are_usages inputs_of_IntegerLessThanNode member_filter member_rec(1) node.hyps(4) node.hyps(6) node.prems(2) not_in_no_val)
-  then show ?case using v1 v2
-    using IntegerLessThanNode node.hyps(5) node.hyps(6) node.prems(3) by fastforce
-next
-  case (ConditionalNode m condition cond trueExp trueVal falseExp falseVal val nid)
-  have trueVal: "g2 m \<turnstile> trueExp (kind g2 trueExp) \<mapsto> IntVal(trueVal)"
-    by (metis (no_types, lifting) ConditionalNode.hyps(3) ConditionalNode.hyps(4) ConditionalNode.hyps(8) ConditionalNode.prems(2) changes.simps eval_usages.simps eval_uses.intros(2) filter_set in_set_member inputs_are_usages inputs_of_ConditionalNode member_filter member_rec(1) not_in_no_val)
-  have falseVal: "g2 m \<turnstile> falseExp (kind g2 falseExp) \<mapsto> IntVal(falseVal)"
-    by (metis (no_types, lifting) ConditionalNode.hyps(5) ConditionalNode.hyps(6) ConditionalNode.hyps(8) ConditionalNode.prems(2) changes.simps eval_usages.simps eval_uses.intros(2) filter_set in_set_member inputs_are_usages inputs_of_ConditionalNode member_filter member_rec(1) not_in_no_val)
-  have cond: "g2 m \<turnstile> condition (kind g2 condition) \<mapsto> IntVal(cond)"
-    by (metis ConditionalNode.hyps(1) ConditionalNode.hyps(2) ConditionalNode.hyps(8) ConditionalNode.prems(2) changes.simps inputs_are_usages inputs_of_ConditionalNode list.set_intros(1) not_in_no_val unchanged_implies_unchanged_inputs)
-  have "g2 m \<turnstile> nid (kind g2 nid) \<mapsto> val"
-    using kind_same trueVal falseVal cond
-    using ConditionalNode.hyps(7) ConditionalNode.hyps(8) ConditionalNode.prems(1) eval.ConditionalNode by fastforce
-  then show ?case
-    by blast
-next
-  case node: (ShortCircuitOrNode m x v1 y v2 val nid)
-  then have "g1 m \<turnstile> x (kind g1 x) \<mapsto> IntVal v1"
-    by blast
-  then have v1: "g2 m \<turnstile> x (kind g2 x) \<mapsto> IntVal v1"
-    by (metis changes.elims(3) inputs_are_usages inputs_of_ShortCircuitOrNode list.set_intros(1) node.hyps(2) node.hyps(6) node.prems(2) not_in_no_val unchanged_implies_unchanged_inputs)
-  have "g1 m \<turnstile> y (kind g1 y) \<mapsto> IntVal v2"
-    using node.hyps(3) by auto
-  then have v2: "g2 m \<turnstile> y (kind g2 y) \<mapsto> IntVal v2"
-    by (metis (no_types, lifting) changes.simps eval_usages.simps eval_uses.intros(2) filter_set in_set_member inputs_are_usages inputs_of_ShortCircuitOrNode member_filter member_rec(1) node.hyps(4) node.hyps(6) node.prems(2) not_in_no_val)
-  then show ?case using v1 v2
-    using eval.ShortCircuitOrNode node.hyps(5) node.hyps(6) node.prems(3) by fastforce
-next
-  case node: (LogicNegationNode m x v1 val nid)
-  then have "g1 m \<turnstile> x (kind g1 x) \<mapsto> IntVal v1"
-    by blast
-  then have v1: "g2 m \<turnstile> x (kind g2 x) \<mapsto> IntVal v1"
-    by (metis changes.elims(3) inputs_are_usages inputs_of_LogicNegationNode list.set_intros(1) node.hyps(2) node.hyps(4) node.prems(2) not_in_no_val unchanged_implies_unchanged_inputs)
-  then show ?case using v1
-    using LogicNegationNode node.hyps(3) node.hyps(4) node.prems(3) by fastforce
-next
-  case (CallNodeEval val m nid start args children)
-  then show ?case sorry
-next
-  case (RefNode m x val nid)
-  then show ?case
-    by (metis changes.elims(3) eval.RefNode inputs_are_usages inputs_of_RefNode list.set_intros(1) not_in_no_val unchanged_implies_unchanged_inputs)
-next
-  case (InvokeNodeEval val m nid callTarget classInit stateDuring stateAfter nex)
-  then show ?case sorry
-next
-  case (SignedDivNode m x v1 y v2 nid zeroCheck frameState nex)
-  then show ?case sorry
-next
-  case (InvokeWithExceptionNodeEval val m nid callTarget classInit stateDuring stateAfter nex exceptionEdge)
-  then show ?case sorry
-next
-  case (NewInstanceNode m nid clazz stateBefore nex)
-  then show ?case
-    by (metis eval.NewInstanceNode)
-qed
-qed
-
-lemma eval_uses_to_changes:
-  assumes "nid \<noteq> nid'"
-  assumes "\<not>(eval_uses g1 nid nid')"
-  assumes "g2 = add_node nid' n g1"
-  shows "\<not>(changes nid g1 g2) \<and> (\<forall> nid' \<in> (eval_usages g1 nid) . \<not>(changes nid' g1 g2))" (is "?P \<and> ?Q")
-proof
-  show ?P
-    using assms(1) assms(3) changes.simps kind_uneffected_uneq by blast
-next
-  show ?Q 
-    by (metis assms(2) assms(3) changes.elims(2) eval_usages.simps filter_set kind_uneffected_uneq member_filter)
-qed
-
-lemma eval_independent:
-  assumes indep: "\<not>(eval_uses g1 nid nid') \<and> nid \<noteq> nid'"
-  assumes g2: "g2 = add_node nid' n g1"
-  assumes v1: "g1 m \<turnstile> nid (kind g1 nid) \<mapsto> v1"
-  shows "g2 m \<turnstile> nid (kind g2 nid) \<mapsto> v1"
-proof -
-  have nid_in: "nid \<in> ids g1"
-    using not_in_no_val v1 by blast
-  then have k: "(kind g1 nid) = (kind g2 nid)"
-    using g2 indep kind_uneffected_uneq by blast
-  show ?thesis
-  proof (cases "is_floating_node (kind g2 nid)")
-    case True
-    then show ?thesis
-      using eval_uses_to_changes indep g2 v1 stay_same
-      by meson
-  next
-    case False
-    then show ?thesis
-      using evalFloating k v1 by fastforce
-  qed
-qed
-
-lemma eval_independent_eq:
-  assumes indep: "\<not>(eval_uses g1 nid nid') \<and> nid \<noteq> nid'"
-  assumes not_in: "nid' \<notin> ids g1"
-  assumes g2: "g2 = add_node nid' n g1"
-  assumes v1: "g1 m \<turnstile> nid (kind g1 nid) \<mapsto> v1"
-  assumes v2: "g2 m \<turnstile> nid (kind g2 nid) \<mapsto> v2"
-  shows "v1 = v2"
-  using eval_independent 
-  by (meson evalDet g2 indep not_in v1 v2)
-
-lemma indep_implies_value:
-  assumes indep: "\<not>(eval_uses g1 nid nid') \<and> nid \<noteq> nid'"
-  assumes not_in: "nid' \<notin> ids g1"
-  assumes g2: "g2 = add_node nid' n g1"
-  assumes v1: "g1 m \<turnstile> nid (kind g1 nid) \<mapsto> v1"
-  shows "\<exists> v2 . (g2 m \<turnstile> nid (kind g2 nid) \<mapsto> v2)"
-proof -
-  obtain v2 where "v2 = v1" by blast
-  have "g2 m \<turnstile> nid (kind g2 nid) \<mapsto> v2"
-    using \<open>v2 = v1\<close> eval_independent g2 indep not_in v1 by blast
-  then show ?thesis using eval_independent
-    by blast
-qed
-
-(*
-lemma eval_independent:
-  assumes fresh: "nid' |\<notin>| fmdom g1"
-  assumes g2: "g2 = fmupd nid' n g1"
-  assumes v1: "g1 m \<turnstile> nid (kind g1 nid) \<mapsto> v1"
-  assumes v2: "g2 m \<turnstile> nid (kind g2 nid) \<mapsto> v2"
-  shows "v1 = v2"
-proof -
-  have eq_kind: "kind g1 nid = kind g2 nid"
-    using fresh g2 v1 by auto
-  have uses: "eval_uses g1 nid = eval_uses g2 nid"
-
-  have uses_g1: "eval_uses g1 nid nid' \<longrightarrow> nid' |\<in>| fmdom g1"
-
-  have uses_g2: "eval_uses g2 nid nid' \<longrightarrow> nid' |\<in>| fmdom g1"
-
-  show ?thesis
-  proof (induction "kind g1 nid")
-*)
-
-
-(*
-lemma in_int_val:
-  assumes "nid \<in> ids g"
-  shows "g m \<turnstile> nid (kind g nid) \<mapsto> IntVal x"
-proof -
-  have kind: "(kind g nid) \<noteq> NoNode"
-    using assms irgraph_dom_x kind.simps apply simp
-    sorry
-  show ?thesis using kind sorry
-qed
-*)
-
-lemma we_can_do_this:
-  assumes "\<not>(\<exists> val . kind g nid = ConstantNode val)"
-  shows "(case kind g nid of ConstantNode condv \<Rightarrow> a | _ \<Rightarrow> b) = b"
-  apply (cases "kind g nid"; auto) using assms
-  by simp
 
 text_raw \<open>\Snip{IfNodeCreate}%\<close>
 lemma if_node_create:
-  assumes cv: "g m \<turnstile> cond (kind g cond) \<mapsto> IntVal cv"
+  assumes cv: "g m \<turnstile> cond (the (kind g cond)) \<mapsto> IntVal cv"
   assumes fresh: "nid \<notin> ids g" 
   assumes gif: "gif = add_node nid (IfNode cond tb fb) g"
   assumes gif_lookup: "gif = gif_prog sig"
@@ -628,31 +200,31 @@ lemma if_node_create:
   shows "\<exists>nid'. (gif_prog sig m \<turnstile> nid \<leadsto> nid') \<and> 
                 (gcreate_prog sig m \<turnstile> nid \<leadsto> nid')"
 text_raw \<open>\EndSnip\<close>
-proof (cases "\<exists> val . kind g cond = ConstantNode val")
+proof (cases "\<exists> val . the (kind g cond) = ConstantNode val")
   case True
   show ?thesis
   proof -
-    obtain val where val: "kind g cond = ConstantNode val"
+    obtain val where val: "the (kind g cond) = ConstantNode val"
       using True by blast
     have cond_exists: "cond \<in> ids g"
-      using not_in_no_val
-      using cv by blast
-    have if_cv: "gif m \<turnstile> cond (kind gif cond) \<mapsto> IntVal val"
+      using breaking_some
+      using cv by auto
+    have if_kind: "kind gif nid = Some (IfNode cond tb fb)"
+      using gif add_node_lookup by simp
+    have if_cv: "gif m \<turnstile> cond (the (kind gif cond)) \<mapsto> IntVal val"
+      using step.IfNode 
       using True eval.ConstantNode gif fresh
-      using kind_uneffected cond_exists
-      using val by presburger
+      using stay_same cond_exists
+      using val sorry
     have if_step: "(gif_prog, sig) \<turnstile> (nid,m,heap) \<rightarrow> (if val_to_bool val then tb else fb,m,heap)"
     proof -
-      have if_kind: "kind gif nid = IfNode cond tb fb"
-        using gif add_implies_kind
-        by blast
       show ?thesis using step.IfNode if_kind if_cv 
         by (simp add: gif_lookup)
     qed
     have create_step: "(gcreate_prog, sig) \<turnstile> (nid,m,heap) \<rightarrow> (if val_to_bool val then tb else fb,m,heap)"
     proof -
-      have create_kind: "kind gcreate nid = create_if g cond tb fb"
-        using gcreate add_implies_kind
+      have create_kind: "kind gcreate nid = Some (create_if g cond tb fb)"
+        using gcreate add_node_lookup
         by blast
       have create_fun: "create_if g cond tb fb = RefNode (if val_to_bool val then tb else fb)"
         using True create_kind val by simp 
@@ -669,37 +241,36 @@ next
   proof -
     have nid': "nid' = (if val_to_bool cv then tb else fb)"
       by (simp add: \<open>nid' = (if val_to_bool cv then tb else fb)\<close>)
-    have gif_kind: "kind gif nid = IfNode cond tb fb"
-      using add_implies_kind gif
+    have gif_kind: "kind gif nid = Some (IfNode cond tb fb)"
+      using add_node_lookup gif
       by blast
     have "nid \<noteq> cond"
-      using cv fresh not_in_no_val by blast
-    obtain cv2 where cv2: "gif m \<turnstile> cond (kind gif cond) \<mapsto> cv2" 
-      using indep_implies_value
+      using cv fresh sorry
+    obtain cv2 where cv2: "gif m \<turnstile> cond (the (kind gif cond)) \<mapsto> cv2" 
       using \<open>nid \<noteq> cond\<close> cv gif indep
-      using fresh by blast
+      using fresh sorry
     then have "IntVal cv = cv2"
-      using indep eval_independent_eq gif cv
+      using indep gif cv
       using \<open>nid \<noteq> cond\<close>
-      using fresh by blast
+      using fresh sorry
     then have eval_gif: "((gif_prog, sig) \<turnstile> (nid,m,heap) \<rightarrow> (nid',m,heap))"
       using step.IfNode gif_kind nid' cv2 
       using gif_lookup by auto
-    have gcreate_kind: "kind gcreate nid = create_if g cond tb fb"
-      using gcreate add_implies_kind
+    have gcreate_kind: "kind gcreate nid = Some (create_if g cond tb fb)"
+      using gcreate add_node_lookup
       by blast
     have eval_gcreate: "(gcreate_prog, sig) \<turnstile> (nid,m,heap) \<rightarrow> (nid',m,heap)"
     proof (cases "tb = fb")
       case True
       have "create_if g cond tb fb = RefNode tb"
-        using not_const True by (cases "kind g cond"; auto)
+        using not_const True by (cases "the (kind g cond)"; auto)
       then show ?thesis
         using True gcreate_kind nid' step.RefNode
         by (simp add: gcreate_lookup)
     next
       case False
       have "create_if g cond tb fb = IfNode cond tb fb"
-        using not_const False by (cases "kind g cond"; auto)
+        using not_const False by (cases "the (kind g cond)"; auto)
       then show ?thesis
         using eval_gif gcreate gif
         using IfNode \<open>IntVal cv = cv2\<close> cv2 gcreate_lookup gif_kind nid' by auto
@@ -710,39 +281,5 @@ next
   show ?thesis using nid_eq Step by blast
 qed
 
-(*
-(cases "kind g y")
-
-      case (ConstantNode yvv)
-      then show ?thesis 
-      proof -
-        have ex: "g m \<turnstile> x (kind g x) \<mapsto> IntVal(xvv)" 
-
-
-proof (cases "kind g x")
-  case "ConstantNode xv"
-  then proof (cases "kind g y")
-  case ConstantNode yv
-  then 
-next
-  case _
-  then
-qed
-*)
-
-(*
-    (case (kind g x) of
-      (ConstantNode xv) \<Rightarrow>
-        (case (kind g y) of
-          (ConstantNode yv) \<Rightarrow> (add_node g (ConstantNode (xv+yv))) |
-          _ \<Rightarrow> (create_add g y x)
-        ) |
-      _ \<Rightarrow> 
-        (case (kind g y) of
-          (ConstantNode 0) \<Rightarrow> (g, x) |
-          _ \<Rightarrow> (add_node g (AddNode x y))
-        )
-    )"
-*)
 
 end
